src/Init/Data/String/Basic.lean
@@ -305,20 +305,20 @@ def next' (s : @& String) (p : @& Pos) (h : ¬ s.atEnd p) : Pos :=
   let c := get s p
   p + c
 
-theorem _root_.Char.size_pos (c : Char) : 0 < c.size := by
+theorem _root_.Char.utf8Size_pos (c : Char) : 0 < c.utf8Size := by
   repeat first | apply iteInduction (motive := (0 < ·)) <;> intros | decide
 
-theorem _root_.Char.size_le_four (c : Char) : c.size ≤ 4 := by
+theorem _root_.Char.utf8Size_le_four (c : Char) : c.utf8Size ≤ 4 := by
   repeat first | apply iteInduction (motive := (· ≤ 4)) <;> intros | decide
 
-@[deprecated Char.size_pos (since := "2026-06-04")] abbrev one_le_csize := Char.size_pos
+@[deprecated Char.utf8Size_pos (since := "2026-06-04")] abbrev one_le_csize := Char.utf8Size_pos
 
 @[simp] theorem pos_lt_eq (p₁ p₂ : Pos) : (p₁ < p₂) = (p₁.1 < p₂.1) := rfl
 
-@[simp] theorem pos_add_char (p : Pos) (c : Char) : (p + c).byteIdx = p.byteIdx + c.size := rfl
+@[simp] theorem pos_add_char (p : Pos) (c : Char) : (p + c).byteIdx = p.byteIdx + c.utf8Size := rfl
 
 theorem lt_next (s : String) (i : Pos) : i.1 < (s.next i).1 :=
-  Nat.add_lt_add_left (Char.size_pos _) _
+  Nat.add_lt_add_left (Char.utf8Size_pos _) _
 
 theorem utf8PrevAux_lt_of_pos : ∀ (cs : List Char) (i p : Pos), p ≠ 0 →
     (utf8PrevAux cs i p).1 < p.1
@@ -328,7 +328,7 @@ theorem utf8PrevAux_lt_of_pos : ∀ (cs : List Char) (i p : Pos), p ≠ 0 →
   | c::cs, i, p, h => by
     simp [utf8PrevAux]
     apply iteInduction (motive := (Pos.byteIdx · < _)) <;> intro h'
-    next => exact h' ▸ Nat.add_lt_add_left (Char.size_pos _) _
+    next => exact h' ▸ Nat.add_lt_add_left (Char.utf8Size_pos _) _
     next => exact utf8PrevAux_lt_of_pos _ _ _ h
 
 theorem prev_lt_of_pos (s : String) (i : Pos) (h : i ≠ 0) : (s.prev i).1 < i.1 := by
@@ -481,7 +481,7 @@ decreasing_by
   focus
     rename_i i₀ j₀ _ eq h'
     rw [show (s.next i₀ - sep.next j₀).1 = (i₀ - j₀).1 by
-      show (_ + Char.size _) - (_ + Char.size _) = _
+      show (_ + Char.utf8Size _) - (_ + Char.utf8Size _) = _
       rw [(beq_iff_eq ..).1 eq, Nat.add_sub_add_right]; rfl]
     right; exact Nat.sub_lt_sub_left
       (Nat.lt_of_le_of_lt (Nat.le_add_right ..) (Nat.gt_of_not_le (mt decide_eq_true h')))
@@ -729,18 +729,18 @@ theorem set_next_add (s : String) (i : Pos) (c : Char) (b₁ b₂)
   simp [next, get, set, endPos, utf8ByteSize] at h ⊢
   rw [Nat.add_comm i.1, Nat.add_assoc] at h ⊢
   let rec foo : ∀ cs a b₁ b₂,
-    (utf8GetAux cs a i).size + b₁ = utf8ByteSize.go cs + b₂ →
-    (utf8GetAux (utf8SetAux c cs a i) a i).size + b₁ = utf8ByteSize.go (utf8SetAux c cs a i) + b₂
+    (utf8GetAux cs a i).utf8Size + b₁ = utf8ByteSize.go cs + b₂ →
+    (utf8GetAux (utf8SetAux c cs a i) a i).utf8Size + b₁ = utf8ByteSize.go (utf8SetAux c cs a i) + b₂
   | [], _, _, _, h => h
   | c'::cs, a, b₁, b₂, h => by
     unfold utf8SetAux
-    apply iteInduction (motive := fun p => (utf8GetAux p a i).size + b₁ = utf8ByteSize.go p + b₂) <;>
+    apply iteInduction (motive := fun p => (utf8GetAux p a i).utf8Size + b₁ = utf8ByteSize.go p + b₂) <;>
       intro h' <;> simp [utf8GetAux, h', utf8ByteSize.go] at h ⊢
     next =>
       rw [Nat.add_assoc, Nat.add_left_comm] at h ⊢; rw [Nat.add_left_cancel h]
     next =>
       rw [Nat.add_assoc] at h ⊢
-      refine foo cs (a + c') b₁ (c'.size + b₂) h
+      refine foo cs (a + c') b₁ (c'.utf8Size + b₂) h
   exact foo s.1 0 _ _ h
 
 theorem mapAux_lemma (s : String) (i : Pos) (c : Char) (h : ¬s.atEnd i) :
@@ -793,7 +793,7 @@ where
     else true
   termination_by stop1.1 - off1.1
   decreasing_by
-    have := Nat.sub_lt_sub_left _h (Nat.add_lt_add_left c₁.size_pos off1.1)
+    have := Nat.sub_lt_sub_left _h (Nat.add_lt_add_left c₁.utf8Size_pos off1.1)
     decreasing_tactic
 
 /-- Return true iff `p` is a prefix of `s` -/
